src/program_proof/mvcc/txn_do_txn.v
@@ -3,16 +3,6 @@ From Perennial.program_proof.mvcc Require Import mvcc_inv txn_common txn_begin t
 Section program.
 Context `{!heapGS Σ, !mvcc_ghostG Σ}.
 
-(*
-Definition spec_body (body : val) (txn : loc) tid r P Q γ τ : iProp Σ :=
-  {{{ own_txn txn tid r γ τ ∗ ⌜P r⌝ ∗ txnmap_ptstos τ r }}}
-    body #txn
-  {{{ (ok : bool), RET #ok;
-      own_txn txn tid r γ τ ∗
-      if ok then ∃ w, ⌜Q r w ∧ dom r = dom w⌝ ∗ txnmap_ptstos τ w else True
-  }}}.
-*)
-
 Definition spec_body
            (body : val) (txn : loc) tid r
            (P : dbmap -> Prop) (Q : dbmap -> dbmap -> Prop)
